lots of updates

src/GZF/KPair.thy
@@ -10,41 +10,112 @@ definition kpair :: "['a,'a] \<Rightarrow> 'a" where
   "kpair a b \<equiv> {{a,b},{a,a}}"
 
 definition is_kpair :: \<open>'a \<Rightarrow> bool\<close>
-  where "is_kpair p = (p : Set \<and> (\<exists>a : SetMem. \<exists>b : SetMem. p = kpair a b))"
+  where "is_kpair p \<equiv> p : SetOf Set \<and> (\<exists>a b. p = kpair a b)"
 
-lemma kpair_typ_set : "kpair : SetMem \<rightarrow> SetMem \<rightarrow> Set" unfolding kpair_def
-  by (rule funI, rule funI, 
-      use upair_set[OF set_setmem[OF upair_set] set_setmem[OF upair_set]] in auto)
+lemma kpair_typ_setof : "kpair : SetMem \<rightarrow> SetMem \<rightarrow> SetOf Set" unfolding kpair_def
+  by (rule funI, rule funI, rule upair_setof[OF upair_set upair_set])
 
-lemmas kpair_set [typ_intro] = funE[OF funE[OF kpair_typ_set]]
+
+lemmas kpair_setof [typ_intro] = funE[OF funE[OF kpair_typ_setof]]
   
+lemma is_kpairI : 
+  assumes "b : SetMem" "c : SetMem"
+  shows "kpair b c : is_kpair"
+  using kpair_setof assms
+  unfolding is_kpair_def has_ty_def by auto
+
+lemma is_kpairE :
+  assumes "p : is_kpair"
+  obtains b c where 
+    "b : SetMem" "c : SetMem" "p = kpair b c"
+proof -
+  from assms obtain b c where
+    "p : SetOf Set" and p_eq:"p = kpair b c"
+    unfolding is_kpair_def has_ty_def by blast
+  hence bb:"{b,b} : SetMem" and bc:"{b,c} : SetMem"
+    using upair_set_setmem[OF setof_set] unfolding kpair_def by auto
+  hence "{b,c} : Set"
+    using setof_mem[OF \<open>p : SetOf Set\<close>] 
+          upairI1[OF bc bb]
+    unfolding \<open>p = kpair b c\<close> kpair_def by auto
+  hence "b : SetMem" "c : SetMem" "p = kpair b c"
+    using upair_set_setmem p_eq by auto
+  thus ?thesis ..
+qed
+
 lemma kpair_iff : 
   assumes "a : SetMem" "b : SetMem" "c : SetMem" "d : SetMem" 
   shows "kpair a b = kpair c d \<longleftrightarrow> a = c \<and> b = d" 
 proof -
   have "upair a b : SetMem" "upair a a : SetMem" "upair c d : SetMem" "upair c c : SetMem" 
     using set_setmem[OF upair_set] assms by auto
-  thus ?thesis unfolding kpair_def using upair_eq_iff assms by metis
+  thus ?thesis unfolding kpair_def using upair_eq_iff assms by fastforce
 qed
-(*FIXME, figure out how to interpret OPair class using Kpairs*)
-interpretation OPair
-  where OPair_default = GZF_default
-    and Pair = is_kpair
-    and pair = kpair
-    and PairMem = SetMem sorry
-(*It seems like when we interpret the pair locale,
-  we don't carry over it's syntax, or the attributes places upon facts.
-  Can this be resolved in any way? 
-  Perhaps using "bundles"?*)
 
+lemma is_kpairD :
+  assumes "kpair b c : is_kpair" 
+  shows "b : SetMem \<and> c : SetMem"
+proof 
+  from assms have
+    kp:"kpair b c : SetOf Set"
+    unfolding is_kpair_def has_ty_def by blast
+  hence bb:"{b,b} : SetMem" and bc:"{b,c} : SetMem"
+    using upair_set_setmem[OF setof_set] unfolding kpair_def by auto
+  hence "{b,c} : Set" using setof_mem[OF kp] upairI1[OF bc bb]
+    unfolding kpair_def by auto
+  thus "b : SetMem" "c : SetMem"
+    using upair_set_setmem by auto
+qed
+
+theorem GZF_OPair :
+  "class.OPair is_kpair kpair SetMem"
+proof
+  show "kpair : SetMem \<rightarrow> SetMem \<rightarrow> is_kpair \<triangle> SetMem"
+  by (rule funI, rule funI, rule intI, rule is_kpairI, auto, 
+      rule set_setmem[OF setof_set[OF kpair_setof]], auto) 
+  
+  show "\<forall>a : SetMem. \<forall>b : SetMem. \<forall>c : SetMem. \<forall>d : SetMem. 
+          (kpair a b = kpair c d) = (a = c \<and> b = d)"
+    unfolding tall_def 
+    using kpair_iff by auto
+
+  show "\<forall>p : is_kpair. \<exists>a b. p = kpair a b"
+    unfolding tall_def 
+    using is_kpairE by meson
+
+  show "\<forall>b. SetMem b \<longleftrightarrow> (\<exists>p : is_kpair. \<exists>c. p = kpair b c \<or> p = kpair c b)"
+  proof (auto)
+    fix b assume "SetMem b"
+    hence "kpair b b : is_kpair"
+      using is_kpairI unfolding has_ty_def by auto
+    thus "\<exists>p : is_kpair. \<exists>c. p = kpair b c \<or> p = kpair c b"
+      by auto
+  next
+    fix b c assume "kpair b c : is_kpair"
+    thus "SetMem b" 
+      using is_kpairD unfolding has_ty_def by auto 
+  next
+    fix b c assume "kpair b c : is_kpair"
+    thus "SetMem c" 
+      using is_kpairD unfolding has_ty_def by auto 
+  qed
+qed
+
+sublocale OPair is_kpair kpair SetMem GZF_default
+  by (intro_locales, rule GZF_OPair)
 
 section \<open>Cartesian Products of Kuratowski Pairs\<close>
 (*Interpret Cartesian Product locale, using GZF for sets, and kpair for ordered pairs. *)
-(* interpretation SetRel 
-  where OPair_default = GZF_default
-    and PairMem = SetMem
-    and pair = kpair 
-  by (unfold_locales, rule kpair_typ)
- *)
 
+lemma kpair_typ_iskpair : "kpair : SetMem \<rightarrow> SetMem \<rightarrow> is_kpair" 
+  by (rule funI, rule funI, rule is_kpairI)
+
+lemma kpair_typ_setmem : "kpair : SetMem \<rightarrow> SetMem \<rightarrow> SetMem" 
+  by (rule funI, rule funI, rule set_setmem[OF setof_set[OF kpair_setof]])
+
+theorem GZF_CartProd :
+  "class.CartProd Set (\<in>) Union Pow \<emptyset> Succ Inf \<R> (\<subseteq>) SetMem SetOf ReplPred is_kpair kpair SetMem"
+  by (intro_locales, unfold_locales, rule kpair_typ_iskpair, rule kpair_typ_setmem)
+
+end
 end
