src/Ordinal/OrdRec.thy
@@ -2,23 +2,6 @@ theory OrdRec
   imports "../GZF/GZF_Base" Ordinal "../Functions/Functions"
 begin
 
-class OrdRec = GZF + Ordinal + 
-  fixes 
-    predSet :: \<open>'a \<Rightarrow> 'a\<close> and 
-    supOrd :: \<open>'a \<Rightarrow> 'a\<close> and
-    OrdRec :: \<open>[['a,'a \<Rightarrow> 'a] \<Rightarrow> 'a, ['a,'a] \<Rightarrow> 'a, 'a, 'a] \<Rightarrow> 'a\<close> and
-    OrdRec_default :: \<open>'a\<close>
-  assumes 
-    predset_typ : "predSet : Ord \<rightarrow> SetOf Ord" and
-    predset_ax :  "\<forall>\<beta> : Ord. \<forall>\<alpha> : Ord. \<alpha> \<in> predSet \<beta> \<longleftrightarrow> \<alpha> < \<beta>" and
-    supord_typ :  "supOrd : SetOf Ord \<rightarrow> Ord" and
-    supord_ax :  "\<forall>x : SetOf Ord. \<forall>\<alpha>. \<alpha> \<in> x \<longrightarrow> \<alpha> \<le> supOrd x" and
-    ordrec_0 :  "\<forall>G. \<forall>F. \<forall>A. OrdRec G F A 0 = A" and
-    ordrec_succ_ax :  "\<forall>G. \<forall>F. \<forall>A. \<forall>b : Ord. 
-       OrdRec G F A (succ b) = F (succ b) (OrdRec G F A b)" and
-    ordrec_lim_ax :  "\<forall>G. \<forall>F. \<forall>A. \<forall>\<mu> : Limit. 
-       OrdRec G F A \<mu> = G \<mu> (\<lambda>j. if j : Ord \<and> j < \<mu> then OrdRec G F A j else OrdRec_default)"                    
-
 syntax
   "_lam_ord" :: "[pttrn, 'a, 'a] => 'a" (\<open>(3\<lambda>_<_./ _)\<close> 10)
 translations
